Improvements to Lib.PrintSequence

lib/fst/Lib.PrintSequence.fst
@@ -22,66 +22,85 @@ let print_lbytes #len b =
   List.iter (fun a -> IO.print_uint8 (u8_to_UInt8 a)) (to_list sb))
 
 
-let print_uint8 x =
+let print_hex_uint8 x =
   IO.print_uint8 (u8_to_UInt8 x)
 
-let print_uint32 x =
+let print_hex_uint32 x =
   IO.print_uint32 (u32_to_UInt32 x)
 
-let print_uint64 x =
+let print_hex_uint64 x =
   IO.print_uint64 (u64_to_UInt64 x)
 
 
-let print_nat8 x =
+let print_dec_uint8 x =
+  IO.print_uint8_dec (u8_to_UInt8 x)
+
+let print_dec_uint32 x =
+  IO.print_uint32_dec (u32_to_UInt32 x)
+
+let print_dec_uint64 x =
+  IO.print_uint64_dec (u64_to_UInt64 x)
+
+
+let print_hex_nat8 x =
   IO.print_uint8 (u8_to_UInt8 (u8 x))
 
-let print_nat32 x =
+let print_hex_nat32 x =
   IO.print_uint32 (u32_to_UInt32 (u32 x))
 
-let print_nat64 x =
+let print_hex_nat64 x =
   IO.print_uint64 (u64_to_UInt64 (u64 x))
 
 
-let print_label_uint8 s x =
+let print_dec_nat8 x =
+  IO.print_uint8_dec (u8_to_UInt8 (u8 x))
+
+let print_dec_nat32 x =
+  IO.print_uint32_dec (u32_to_UInt32 (u32 x))
+
+let print_dec_nat64 x =
+  IO.print_uint64_dec (u64_to_UInt64 (u64 x))
+
+
+let print_label_hex_uint8 s x =
   IO.print_string s;
   IO.print_string ": ";
-  print_uint8 x;
+  print_hex_uint8 x;
   IO.print_string "\n"
 
-let print_label_uint32 s x =
+let print_label_hex_uint32 s x =
   IO.print_string s;
   IO.print_string ": ";
-  print_uint32 x;
+  print_hex_uint32 x;
   IO.print_string "\n"
 
-let print_label_uint64 s x =
+let print_label_hex_uint64 s x =
   IO.print_string s;
   IO.print_string ": ";
-  print_uint64 x;
+  print_hex_uint64 x;
   IO.print_string "\n"
 
-let print_label_nat8 s x =
+let print_label_dec_nat8 s x =
   IO.print_string s;
   IO.print_string ": ";
-  print_nat8 x;
+  print_dec_nat8 x;
   IO.print_string "\n"
 
-let print_label_nat32 s x =
+let print_label_dec_nat32 s x =
   IO.print_string s;
   IO.print_string ": ";
-  print_nat32 x;
+  print_dec_nat32 x;
   IO.print_string "\n"
 
-let print_label_nat64 s x =
+let print_label_dec_nat64 s x =
   IO.print_string s;
   IO.print_string ": ";
-  print_nat64 x;
+  print_dec_nat64 x;
   IO.print_string "\n"
-
 
 let print_compare len expected result =
   IO.print_string "\n\nResult:   ";
-  List.iter (fun a -> print_uint8 a) (to_list result);
+  List.iter (fun a -> print_hex_uint8 a) (to_list result);
   IO.print_string "\nExpected: ";
-  List.iter (fun a -> print_uint8 a) (to_list expected);
+  List.iter (fun a -> print_hex_uint8 a) (to_list expected);
   for_all2 (fun a b -> uint_to_nat #U8 a = uint_to_nat #U8 b) expected result
